Examples with quantified formulas.

Formula.v
@@ -12,6 +12,17 @@ Section formula.
   | FNeg : formula X -> formula X
   | FAll : formula X⁺ -> formula X.
    
+  Definition FExists X (φ : formula X⁺) : formula X := FNeg _ (FAll _ (FNeg _ φ)).
+
 End formula.
 
 Arguments formula : clear implicits.
+Arguments FPred [Σ X] R _.
+Arguments FIndPred [Σ X] R _.
+Arguments FImp [Σ X] _ _.
+Arguments FNeg [Σ X] _.
+Arguments FAll [Σ X] _.
+Arguments FExists [Σ X] _.
+
+
+
